latest changes

examples/mk_acc.c
@@ -1,5 +1,6 @@
 #include <stddef.h>
 
+
 extern void free(void *p);
 extern void *malloc(size_t size);
 
