examples/verif_dll_dupleton.v
@@ -27,7 +27,7 @@ Fixpoint dll (x: val) (z: val) (s: (list Z)) (self_card: dll_card) {struct self_
       EX v : Z,
       EX s1 : (list Z),
       EX w : val,
- !!(Int.min_signed <= v <= Int.max_signed) && !!(~ ((x : val) = nullval)) && !!((s : list Z) = (([(v : Z)] : list Z) ++ (s1 : list Z))) && (data_at Tsh (tarray (Tunion _sslval noattr) 3) [(inl ((Vint (Int.repr v)) : val)); (inr (w : val)); (inr (z : val))] (x : val)) * (dll (w : val) (x : val) (s1 : list Z) (_alpha_513 : dll_card))
+ !!(Int.min_signed <= v <= Int.max_signed) && !!(is_pointer_or_null w) && !!(~ ((x : val) = nullval)) && !!((s : list Z) = (([(v : Z)] : list Z) ++ (s1 : list Z))) && (data_at Tsh (tarray (Tunion _sslval noattr) 3) [(inl ((Vint (Int.repr v)) : val)); (inr (w : val)); (inr (z : val))] (x : val)) * (dll (w : val) (x : val) (s1 : list Z) (_alpha_513 : dll_card))
 end.
 
 Inductive sll_card : Set :=
@@ -40,7 +40,7 @@ Fixpoint sll (x: val) (s: (list Z)) (self_card: sll_card) {struct self_card} : m
       EX v : Z,
       EX s1 : (list Z),
       EX nxt : val,
- !!(Int.min_signed <= v <= Int.max_signed) && !!(~ ((x : val) = nullval)) && !!((s : list Z) = (([(v : Z)] : list Z) ++ (s1 : list Z))) && (data_at Tsh (tarray (Tunion _sslval noattr) 2) [(inl ((Vint (Int.repr v)) : val)); (inr (nxt : val))] (x : val)) * (sll (nxt : val) (s1 : list Z) (_alpha_514 : sll_card))
+ !!(Int.min_signed <= v <= Int.max_signed) && !!(is_pointer_or_null nxt) && !!(~ ((x : val) = nullval)) && !!((s : list Z) = (([(v : Z)] : list Z) ++ (s1 : list Z))) && (data_at Tsh (tarray (Tunion _sslval noattr) 2) [(inl ((Vint (Int.repr v)) : val)); (inr (nxt : val))] (x : val)) * (sll (nxt : val) (s1 : list Z) (_alpha_514 : sll_card))
 end.
 
 
@@ -55,34 +55,34 @@ Definition dll_dupleton_spec :=
    EX _alpha_515: dll_card,
    EX elems: (list Z),
    EX z: val,
-   PROP( ((elems : list Z) = ([(force_signed_int (x : val)); (force_signed_int (y : val))] : list Z)) )
+   PROP( ((elems : list Z) = ([(force_signed_int (x : val)); (force_signed_int (y : val))] : list Z)); is_pointer_or_null((z : val)) )
    LOCAL()
    SEP ((data_at Tsh (tarray (Tunion _sslval noattr) 1) [(inr (z : val))] (r : val)); (dll (z : val) nullval (elems : list Z) (_alpha_515 : dll_card))).
 
-Lemma dll_x_valid_pointerP x z s self_card: dll x z s self_card |-- valid_pointer x. Proof. Admitted.
+Lemma dll_x_valid_pointerP x z s self_card: dll x z s self_card |-- valid_pointer x. Proof. destruct self_card; simpl; entailer;  entailer!; eauto. Qed.
 Hint Resolve dll_x_valid_pointerP : valid_pointer.
-Lemma dll_z_valid_pointerP x z s self_card: dll x z s self_card |-- valid_pointer z. Proof. Admitted.
-Hint Resolve dll_z_valid_pointerP : valid_pointer.
 Lemma dll_local_factsP x z s self_card :
-  dll x z s self_card|-- !!(((((x : val) = nullval)) -> (self_card = dll_card_0))/\(((~ ((x : val) = nullval))) -> (exists _alpha_513, self_card = dll_card_1 _alpha_513))/\is_pointer_or_null((x : val))/\is_pointer_or_null((z : val))). Proof. Admitted.
+  dll x z s self_card|-- !!(((((x : val) = nullval)) -> (self_card = dll_card_0))/\(((~ ((x : val) = nullval))) -> (exists _alpha_513, self_card = dll_card_1 _alpha_513))/\is_pointer_or_null((x : val))).
+ Proof.  destruct self_card;  simpl; entailer; saturate_local; apply prop_right; eauto. Qed.
 Hint Resolve dll_local_factsP : saturate_local.
 Lemma unfold_dll_card_0  (x: val) (z: val) (s: (list Z)) : dll x z s (dll_card_0 ) =  !!((x : val) = nullval) && !!((s : list Z) = ([] : list Z)) && emp. Proof. auto. Qed.
 Lemma unfold_dll_card_1 (_alpha_513 : dll_card) (x: val) (z: val) (s: (list Z)) : dll x z s (dll_card_1 _alpha_513) = 
       EX v : Z,
       EX s1 : (list Z),
       EX w : val,
- !!(Int.min_signed <= v <= Int.max_signed) && !!(~ ((x : val) = nullval)) && !!((s : list Z) = (([(v : Z)] : list Z) ++ (s1 : list Z))) && (data_at Tsh (tarray (Tunion _sslval noattr) 3) [(inl ((Vint (Int.repr v)) : val)); (inr (w : val)); (inr (z : val))] (x : val)) * (dll (w : val) (x : val) (s1 : list Z) (_alpha_513 : dll_card)). Proof. auto. Qed.
-Lemma sll_x_valid_pointerP x s self_card: sll x s self_card |-- valid_pointer x. Proof. Admitted.
+ !!(Int.min_signed <= v <= Int.max_signed) && !!(is_pointer_or_null w) && !!(~ ((x : val) = nullval)) && !!((s : list Z) = (([(v : Z)] : list Z) ++ (s1 : list Z))) && (data_at Tsh (tarray (Tunion _sslval noattr) 3) [(inl ((Vint (Int.repr v)) : val)); (inr (w : val)); (inr (z : val))] (x : val)) * (dll (w : val) (x : val) (s1 : list Z) (_alpha_513 : dll_card)). Proof. auto. Qed.
+Lemma sll_x_valid_pointerP x s self_card: sll x s self_card |-- valid_pointer x. Proof. destruct self_card; simpl; entailer;  entailer!; eauto. Qed.
 Hint Resolve sll_x_valid_pointerP : valid_pointer.
 Lemma sll_local_factsP x s self_card :
-  sll x s self_card|-- !!(((((x : val) = nullval)) -> (self_card = sll_card_0))/\(((~ ((x : val) = nullval))) -> (exists _alpha_514, self_card = sll_card_1 _alpha_514))/\is_pointer_or_null((x : val))). Proof. Admitted.
+  sll x s self_card|-- !!(((((x : val) = nullval)) -> (self_card = sll_card_0))/\(((~ ((x : val) = nullval))) -> (exists _alpha_514, self_card = sll_card_1 _alpha_514))/\is_pointer_or_null((x : val))).
+ Proof.  destruct self_card;  simpl; entailer; saturate_local; apply prop_right; eauto. Qed.
 Hint Resolve sll_local_factsP : saturate_local.
 Lemma unfold_sll_card_0  (x: val) (s: (list Z)) : sll x s (sll_card_0 ) =  !!((x : val) = nullval) && !!((s : list Z) = ([] : list Z)) && emp. Proof. auto. Qed.
 Lemma unfold_sll_card_1 (_alpha_514 : sll_card) (x: val) (s: (list Z)) : sll x s (sll_card_1 _alpha_514) = 
       EX v : Z,
       EX s1 : (list Z),
       EX nxt : val,
- !!(Int.min_signed <= v <= Int.max_signed) && !!(~ ((x : val) = nullval)) && !!((s : list Z) = (([(v : Z)] : list Z) ++ (s1 : list Z))) && (data_at Tsh (tarray (Tunion _sslval noattr) 2) [(inl ((Vint (Int.repr v)) : val)); (inr (nxt : val))] (x : val)) * (sll (nxt : val) (s1 : list Z) (_alpha_514 : sll_card)). Proof. auto. Qed.
+ !!(Int.min_signed <= v <= Int.max_signed) && !!(is_pointer_or_null nxt) && !!(~ ((x : val) = nullval)) && !!((s : list Z) = (([(v : Z)] : list Z) ++ (s1 : list Z))) && (data_at Tsh (tarray (Tunion _sslval noattr) 2) [(inl ((Vint (Int.repr v)) : val)); (inr (nxt : val))] (x : val)) * (sll (nxt : val) (s1 : list Z) (_alpha_514 : sll_card)). Proof. auto. Qed.
 Definition Gprog : funspecs :=
   ltac:(with_library prog [dll_dupleton_spec; malloc_spec]).
 
@@ -111,17 +111,17 @@ Exists (dll_card_1 (dll_card_1 (dll_card_0  : dll_card) : dll_card) : dll_card).
 Exists ([(x : Z); (y : Z)] : list Z).
 Exists (z2 : val).
 ssl_entailer.
-ssl_rewrite_last (unfold_dll_card_1 (dll_card_1 (dll_card_0  : dll_card) : dll_card)).
+rewrite (unfold_dll_card_1 (dll_card_1 (dll_card_0  : dll_card) : dll_card)) at 1.
 Exists (x : Z).
 Exists (([(y : Z)] : list Z) ++ ([] : list Z)).
 Exists (wz2 : val).
 ssl_entailer.
-ssl_rewrite_last (unfold_dll_card_1 (dll_card_0  : dll_card)).
+rewrite (unfold_dll_card_1 (dll_card_0  : dll_card)) at 1.
 Exists (y : Z).
 Exists ([] : list Z).
 Exists nullval.
 ssl_entailer.
-ssl_rewrite_last (unfold_dll_card_0 ).
+rewrite (unfold_dll_card_0 ) at 1.
 ssl_entailer.
 
 Qed.
