examples/verif_sll_append.v
@@ -15,7 +15,7 @@ Fixpoint sll (x: val) (s: (list Z)) (self_card: sll_card) {struct self_card} : m
       EX v : Z,
       EX s1 : (list Z),
       EX nxt : val,
- !!(Int.min_signed <= v <= Int.max_signed) && !!(~ ((x : val) = nullval)) && !!((s : list Z) = (([(v : Z)] : list Z) ++ (s1 : list Z))) && (data_at Tsh (tarray (Tunion _sslval noattr) 2) [(inl ((Vint (Int.repr v)) : val)); (inr (nxt : val))] (x : val)) * (sll (nxt : val) (s1 : list Z) (_alpha_513 : sll_card))
+ !!(Int.min_signed <= v <= Int.max_signed) && !!(is_pointer_or_null nxt) && !!(~ ((x : val) = nullval)) && !!((s : list Z) = (([(v : Z)] : list Z) ++ (s1 : list Z))) && (data_at Tsh (tarray (Tunion _sslval noattr) 2) [(inl ((Vint (Int.repr v)) : val)); (inr (nxt : val))] (x : val)) * (sll (nxt : val) (s1 : list Z) (_alpha_513 : sll_card))
 end.
 
 
@@ -25,26 +25,27 @@ Definition sll_append_spec :=
    PRE [ (tptr (Tunion _sslval noattr)), (tptr (Tunion _sslval noattr)) ]
    PROP( is_pointer_or_null((x1 : val)); is_pointer_or_null((r : val)); is_pointer_or_null((x2 : val)) )
    PARAMS(x1; r)
-   SEP ((data_at Tsh (tarray (Tunion _sslval noattr) 1) [(inr (x2 : val))] (r : val)); (sll (x2 : val) (s2 : list Z) (_alpha_515 : sll_card)); (sll (x1 : val) (s1 : list Z) (_alpha_514 : sll_card)))
+   SEP ((data_at Tsh (tarray (Tunion _sslval noattr) 1) [(inr (x2 : val))] (r : val)); (sll (x1 : val) (s1 : list Z) (_alpha_514 : sll_card)); (sll (x2 : val) (s2 : list Z) (_alpha_515 : sll_card)))
    POST[ tvoid ]
    EX y: val,
    EX s: (list Z),
    EX _alpha_516: sll_card,
-   PROP( ((s : list Z) = ((s1 : list Z) ++ (s2 : list Z))) )
+   PROP( ((s : list Z) = ((s1 : list Z) ++ (s2 : list Z))); is_pointer_or_null((y : val)) )
    LOCAL()
    SEP ((data_at Tsh (tarray (Tunion _sslval noattr) 1) [(inr (y : val))] (r : val)); (sll (y : val) (s : list Z) (_alpha_516 : sll_card))).
 
-Lemma sll_x_valid_pointerP x s self_card: sll x s self_card |-- valid_pointer x. Proof. Admitted.
+Lemma sll_x_valid_pointerP x s self_card: sll x s self_card |-- valid_pointer x. Proof. destruct self_card; simpl; entailer;  entailer!; eauto. Qed.
 Hint Resolve sll_x_valid_pointerP : valid_pointer.
 Lemma sll_local_factsP x s self_card :
-  sll x s self_card|-- !!(((((x : val) = nullval)) -> (self_card = sll_card_0))/\(((~ ((x : val) = nullval))) -> (exists _alpha_513, self_card = sll_card_1 _alpha_513))/\is_pointer_or_null((x : val))). Proof. Admitted.
+  sll x s self_card|-- !!(((((x : val) = nullval)) -> (self_card = sll_card_0))/\(((~ ((x : val) = nullval))) -> (exists _alpha_513, self_card = sll_card_1 _alpha_513))/\is_pointer_or_null((x : val))).
+ Proof.  destruct self_card;  simpl; entailer; saturate_local; apply prop_right; eauto. Qed.
 Hint Resolve sll_local_factsP : saturate_local.
 Lemma unfold_sll_card_0  (x: val) (s: (list Z)) : sll x s (sll_card_0 ) =  !!((x : val) = nullval) && !!((s : list Z) = ([] : list Z)) && emp. Proof. auto. Qed.
 Lemma unfold_sll_card_1 (_alpha_513 : sll_card) (x: val) (s: (list Z)) : sll x s (sll_card_1 _alpha_513) = 
       EX v : Z,
       EX s1 : (list Z),
       EX nxt : val,
- !!(Int.min_signed <= v <= Int.max_signed) && !!(~ ((x : val) = nullval)) && !!((s : list Z) = (([(v : Z)] : list Z) ++ (s1 : list Z))) && (data_at Tsh (tarray (Tunion _sslval noattr) 2) [(inl ((Vint (Int.repr v)) : val)); (inr (nxt : val))] (x : val)) * (sll (nxt : val) (s1 : list Z) (_alpha_513 : sll_card)). Proof. auto. Qed.
+ !!(Int.min_signed <= v <= Int.max_signed) && !!(is_pointer_or_null nxt) && !!(~ ((x : val) = nullval)) && !!((s : list Z) = (([(v : Z)] : list Z) ++ (s1 : list Z))) && (data_at Tsh (tarray (Tunion _sslval noattr) 2) [(inl ((Vint (Int.repr v)) : val)); (inr (nxt : val))] (x : val)) * (sll (nxt : val) (s1 : list Z) (_alpha_513 : sll_card)). Proof. auto. Qed.
 Definition Gprog : funspecs :=
   ltac:(with_library prog [sll_append_spec]).
 
@@ -95,7 +96,7 @@ Exists (x1 : val).
 Exists ((([(vx12 : Z)] : list Z) ++ (s1x1 : list Z)) ++ (s2 : list Z)).
 Exists (sll_card_1 (_alpha_5161 : sll_card) : sll_card).
 ssl_entailer.
-ssl_rewrite_last (unfold_sll_card_1 (_alpha_5161 : sll_card)).
+rewrite (unfold_sll_card_1 (_alpha_5161 : sll_card)) at 1.
 Exists (vx12 : Z).
 Exists ((s1x1 : list Z) ++ (s2 : list Z)).
 Exists (y12 : val).
