examples/verif_sll_free.v
@@ -27,7 +27,7 @@ Fixpoint sll (x: val) (s: (list Z)) (self_card: sll_card) {struct self_card} : m
       EX v : Z,
       EX s1 : (list Z),
       EX nxt : val,
- !!(Int.min_signed <= v <= Int.max_signed) && !!(~ ((x : val) = nullval)) && !!((s : list Z) = (([(v : Z)] : list Z) ++ (s1 : list Z))) && (data_at Tsh (tarray (Tunion _sslval noattr) 2) [(inl ((Vint (Int.repr v)) : val)); (inr (nxt : val))] (x : val)) * (sll (nxt : val) (s1 : list Z) (_alpha_513 : sll_card))
+ !!(Int.min_signed <= v <= Int.max_signed) && !!(is_pointer_or_null nxt) && !!(~ ((x : val) = nullval)) && !!((s : list Z) = (([(v : Z)] : list Z) ++ (s1 : list Z))) && (data_at Tsh (tarray (Tunion _sslval noattr) 2) [(inl ((Vint (Int.repr v)) : val)); (inr (nxt : val))] (x : val)) * (sll (nxt : val) (s1 : list Z) (_alpha_513 : sll_card))
 end.
 
 
@@ -43,17 +43,18 @@ Definition sll_free_spec :=
    LOCAL()
    SEP ().
 
-Lemma sll_x_valid_pointerP x s self_card: sll x s self_card |-- valid_pointer x. Proof. Admitted.
+Lemma sll_x_valid_pointerP x s self_card: sll x s self_card |-- valid_pointer x. Proof. destruct self_card; simpl; entailer;  entailer!; eauto. Qed.
 Hint Resolve sll_x_valid_pointerP : valid_pointer.
 Lemma sll_local_factsP x s self_card :
-  sll x s self_card|-- !!(((((x : val) = nullval)) -> (self_card = sll_card_0))/\(((~ ((x : val) = nullval))) -> (exists _alpha_513, self_card = sll_card_1 _alpha_513))/\is_pointer_or_null((x : val))). Proof. Admitted.
+  sll x s self_card|-- !!(((((x : val) = nullval)) -> (self_card = sll_card_0))/\(((~ ((x : val) = nullval))) -> (exists _alpha_513, self_card = sll_card_1 _alpha_513))/\is_pointer_or_null((x : val))).
+ Proof.  destruct self_card;  simpl; entailer; saturate_local; apply prop_right; eauto. Qed.
 Hint Resolve sll_local_factsP : saturate_local.
 Lemma unfold_sll_card_0  (x: val) (s: (list Z)) : sll x s (sll_card_0 ) =  !!((x : val) = nullval) && !!((s : list Z) = ([] : list Z)) && emp. Proof. auto. Qed.
 Lemma unfold_sll_card_1 (_alpha_513 : sll_card) (x: val) (s: (list Z)) : sll x s (sll_card_1 _alpha_513) = 
       EX v : Z,
       EX s1 : (list Z),
       EX nxt : val,
- !!(Int.min_signed <= v <= Int.max_signed) && !!(~ ((x : val) = nullval)) && !!((s : list Z) = (([(v : Z)] : list Z) ++ (s1 : list Z))) && (data_at Tsh (tarray (Tunion _sslval noattr) 2) [(inl ((Vint (Int.repr v)) : val)); (inr (nxt : val))] (x : val)) * (sll (nxt : val) (s1 : list Z) (_alpha_513 : sll_card)). Proof. auto. Qed.
+ !!(Int.min_signed <= v <= Int.max_signed) && !!(is_pointer_or_null nxt) && !!(~ ((x : val) = nullval)) && !!((s : list Z) = (([(v : Z)] : list Z) ++ (s1 : list Z))) && (data_at Tsh (tarray (Tunion _sslval noattr) 2) [(inl ((Vint (Int.repr v)) : val)); (inr (nxt : val))] (x : val)) * (sll (nxt : val) (s1 : list Z) (_alpha_513 : sll_card)). Proof. auto. Qed.
 Definition Gprog : funspecs :=
   ltac:(with_library prog [sll_free_spec; free_spec]).
 
