examples/verif_sll_max.v
@@ -17,7 +17,7 @@ Fixpoint sll (x: val) (len: Z) (lo: Z) (hi: Z) (self_card: sll_card) {struct sel
       EX len1 : Z,
       EX hi1 : Z,
       EX lo1 : Z,
- !!(Int.min_signed <= v <= Int.max_signed) && !!(Int.min_signed <= len1 <= Int.max_signed) && !!(Int.min_signed <= hi1 <= Int.max_signed) && !!(Int.min_signed <= lo1 <= Int.max_signed) && !!(~ ((x : val) = nullval)) && !!(0 <= (len1 : Z)) && !!(0 <= (v : Z)) && !!((hi : Z) = (if (Z.leb (hi1 : Z) (v : Z)) then (v : Z) else (hi1 : Z))) && !!((len : Z) = (1 + (len1 : Z))) && !!((lo : Z) = (if (Z.leb (v : Z) (lo1 : Z)) then (v : Z) else (lo1 : Z))) && !!((v : Z) <= 7) && (data_at Tsh (tarray (Tunion _sslval noattr) 2) [(inl ((Vint (Int.repr v)) : val)); (inr (nxt : val))] (x : val)) * (sll (nxt : val) (len1 : Z) (lo1 : Z) (hi1 : Z) (_alpha_513 : sll_card))
+ !!(Int.min_signed <= v <= Int.max_signed) && !!(is_pointer_or_null nxt) && !!(Int.min_signed <= len1 <= Int.max_signed) && !!(Int.min_signed <= hi1 <= Int.max_signed) && !!(Int.min_signed <= lo1 <= Int.max_signed) && !!(~ ((x : val) = nullval)) && !!(0 <= (len1 : Z)) && !!(0 <= (v : Z)) && !!((hi : Z) = (if (Z.leb (hi1 : Z) (v : Z)) then (v : Z) else (hi1 : Z))) && !!((len : Z) = (1 + (len1 : Z))) && !!((lo : Z) = (if (Z.leb (v : Z) (lo1 : Z)) then (v : Z) else (lo1 : Z))) && !!((v : Z) <= 7) && (data_at Tsh (tarray (Tunion _sslval noattr) 2) [(inl ((Vint (Int.repr v)) : val)); (inr (nxt : val))] (x : val)) * (sll (nxt : val) (len1 : Z) (lo1 : Z) (hi1 : Z) (_alpha_513 : sll_card))
 end.
 
 
@@ -34,10 +34,11 @@ Definition sll_max_spec :=
    LOCAL()
    SEP ((data_at Tsh (tarray (Tunion _sslval noattr) 1) [(inl ((Vint (Int.repr hi)) : val))] (r : val)); (sll (x : val) (n : Z) (lo : Z) (hi : Z) (_alpha_515 : sll_card))).
 
-Lemma sll_x_valid_pointerP x len lo hi self_card: sll x len lo hi self_card |-- valid_pointer x. Proof. Admitted.
+Lemma sll_x_valid_pointerP x len lo hi self_card: sll x len lo hi self_card |-- valid_pointer x. Proof. destruct self_card; simpl; entailer;  entailer!; eauto. Qed.
 Hint Resolve sll_x_valid_pointerP : valid_pointer.
 Lemma sll_local_factsP x len lo hi self_card :
-  sll x len lo hi self_card|-- !!(((((x : val) = nullval)) -> (self_card = sll_card_0))/\(((~ ((x : val) = nullval))) -> (exists _alpha_513, self_card = sll_card_1 _alpha_513))/\is_pointer_or_null((x : val))). Proof. Admitted.
+  sll x len lo hi self_card|-- !!(((((x : val) = nullval)) -> (self_card = sll_card_0))/\(((~ ((x : val) = nullval))) -> (exists _alpha_513, self_card = sll_card_1 _alpha_513))/\is_pointer_or_null((x : val))).
+ Proof.  destruct self_card;  simpl; entailer; saturate_local; apply prop_right; eauto. Qed.
 Hint Resolve sll_local_factsP : saturate_local.
 Lemma unfold_sll_card_0  (x: val) (len: Z) (lo: Z) (hi: Z) : sll x len lo hi (sll_card_0 ) =  !!((x : val) = nullval) && !!((hi : Z) = 0) && !!((len : Z) = 0) && !!((lo : Z) = 7) && emp. Proof. auto. Qed.
 Lemma unfold_sll_card_1 (_alpha_513 : sll_card) (x: val) (len: Z) (lo: Z) (hi: Z) : sll x len lo hi (sll_card_1 _alpha_513) = 
@@ -46,7 +47,7 @@ Lemma unfold_sll_card_1 (_alpha_513 : sll_card) (x: val) (len: Z) (lo: Z) (hi: Z
       EX len1 : Z,
       EX hi1 : Z,
       EX lo1 : Z,
- !!(Int.min_signed <= v <= Int.max_signed) && !!(Int.min_signed <= len1 <= Int.max_signed) && !!(Int.min_signed <= hi1 <= Int.max_signed) && !!(Int.min_signed <= lo1 <= Int.max_signed) && !!(~ ((x : val) = nullval)) && !!(0 <= (len1 : Z)) && !!(0 <= (v : Z)) && !!((hi : Z) = (if (Z.leb (hi1 : Z) (v : Z)) then (v : Z) else (hi1 : Z))) && !!((len : Z) = (1 + (len1 : Z))) && !!((lo : Z) = (if (Z.leb (v : Z) (lo1 : Z)) then (v : Z) else (lo1 : Z))) && !!((v : Z) <= 7) && (data_at Tsh (tarray (Tunion _sslval noattr) 2) [(inl ((Vint (Int.repr v)) : val)); (inr (nxt : val))] (x : val)) * (sll (nxt : val) (len1 : Z) (lo1 : Z) (hi1 : Z) (_alpha_513 : sll_card)). Proof. auto. Qed.
+ !!(Int.min_signed <= v <= Int.max_signed) && !!(is_pointer_or_null nxt) && !!(Int.min_signed <= len1 <= Int.max_signed) && !!(Int.min_signed <= hi1 <= Int.max_signed) && !!(Int.min_signed <= lo1 <= Int.max_signed) && !!(~ ((x : val) = nullval)) && !!(0 <= (len1 : Z)) && !!(0 <= (v : Z)) && !!((hi : Z) = (if (Z.leb (hi1 : Z) (v : Z)) then (v : Z) else (hi1 : Z))) && !!((len : Z) = (1 + (len1 : Z))) && !!((lo : Z) = (if (Z.leb (v : Z) (lo1 : Z)) then (v : Z) else (lo1 : Z))) && !!((v : Z) <= 7) && (data_at Tsh (tarray (Tunion _sslval noattr) 2) [(inl ((Vint (Int.repr v)) : val)); (inr (nxt : val))] (x : val)) * (sll (nxt : val) (len1 : Z) (lo1 : Z) (hi1 : Z) (_alpha_513 : sll_card)). Proof. auto. Qed.
 Definition Gprog : funspecs :=
   ltac:(with_library prog [sll_max_spec]).
 
@@ -70,7 +71,7 @@ forward.
 forward; entailer!.
 Exists (sll_card_0  : sll_card).
 ssl_entailer.
-ssl_rewrite_last (unfold_sll_card_0 ).
+rewrite (unfold_sll_card_0 ) at 1.
 ssl_entailer.
 
 }
@@ -100,7 +101,7 @@ forward.
 forward; entailer!.
 Exists (sll_card_1 (_alpha_5151 : sll_card) : sll_card).
 ssl_entailer.
-ssl_rewrite_last (unfold_sll_card_1 (_alpha_5151 : sll_card)).
+rewrite (unfold_sll_card_1 (_alpha_5151 : sll_card)) at 1.
 Exists (vx2 : Z).
 Exists (nxtx2 : val).
 Exists (len1x : Z).
