examples/verif_tree_copy.v
@@ -29,7 +29,7 @@ Fixpoint tree (x: val) (s: (list Z)) (self_card: tree_card) {struct self_card} :
       EX r : val,
       EX s1 : (list Z),
       EX l : val,
- !!(Int.min_signed <= v <= Int.max_signed) && !!(~ ((x : val) = nullval)) && !!((s : list Z) = ((([(v : Z)] : list Z) ++ (s1 : list Z)) ++ (s2 : list Z))) && (data_at Tsh (tarray (Tunion _sslval noattr) 3) [(inl ((Vint (Int.repr v)) : val)); (inr (l : val)); (inr (r : val))] (x : val)) * (tree (r : val) (s2 : list Z) (_alpha_514 : tree_card)) * (tree (l : val) (s1 : list Z) (_alpha_513 : tree_card))
+ !!(Int.min_signed <= v <= Int.max_signed) && !!(is_pointer_or_null r) && !!(is_pointer_or_null l) && !!(~ ((x : val) = nullval)) && !!((s : list Z) = ((([(v : Z)] : list Z) ++ (s1 : list Z)) ++ (s2 : list Z))) && (data_at Tsh (tarray (Tunion _sslval noattr) 3) [(inl ((Vint (Int.repr v)) : val)); (inr (l : val)); (inr (r : val))] (x : val)) * (tree (l : val) (s1 : list Z) (_alpha_513 : tree_card)) * (tree (r : val) (s2 : list Z) (_alpha_514 : tree_card))
 end.
 
 Inductive treeN_card : Set :=
@@ -44,7 +44,7 @@ Fixpoint treeN (x: val) (n: Z) (self_card: treeN_card) {struct self_card} : mpre
       EX r : val,
       EX n2 : Z,
       EX l : val,
- !!(Int.min_signed <= n1 <= Int.max_signed) && !!(Int.min_signed <= n2 <= Int.max_signed) && !!(~ ((x : val) = nullval)) && !!(0 <= (n1 : Z)) && !!(0 <= (n2 : Z)) && !!((n : Z) = ((1 + (n1 : Z)) + (n2 : Z))) && (data_at Tsh (tarray (Tunion _sslval noattr) 3) [(inr (v : val)); (inr (l : val)); (inr (r : val))] (x : val)) * (treeN (r : val) (n2 : Z) (_alpha_516 : treeN_card)) * (treeN (l : val) (n1 : Z) (_alpha_515 : treeN_card))
+ !!(Int.min_signed <= n1 <= Int.max_signed) && !!(is_pointer_or_null v) && !!(is_pointer_or_null r) && !!(Int.min_signed <= n2 <= Int.max_signed) && !!(is_pointer_or_null l) && !!(~ ((x : val) = nullval)) && !!(0 <= (n1 : Z)) && !!(0 <= (n2 : Z)) && !!((n : Z) = ((1 + (n1 : Z)) + (n2 : Z))) && (data_at Tsh (tarray (Tunion _sslval noattr) 3) [(inr (v : val)); (inr (l : val)); (inr (r : val))] (x : val)) * (treeN (l : val) (n1 : Z) (_alpha_515 : treeN_card)) * (treeN (r : val) (n2 : Z) (_alpha_516 : treeN_card))
 end.
 
 Inductive sll_card : Set :=
@@ -57,7 +57,7 @@ Fixpoint sll (x: val) (s: (list Z)) (self_card: sll_card) {struct self_card} : m
       EX v : Z,
       EX s1 : (list Z),
       EX nxt : val,
- !!(Int.min_signed <= v <= Int.max_signed) && !!(~ ((x : val) = nullval)) && !!((s : list Z) = (([(v : Z)] : list Z) ++ (s1 : list Z))) && (data_at Tsh (tarray (Tunion _sslval noattr) 2) [(inl ((Vint (Int.repr v)) : val)); (inr (nxt : val))] (x : val)) * (sll (nxt : val) (s1 : list Z) (_alpha_517 : sll_card))
+ !!(Int.min_signed <= v <= Int.max_signed) && !!(is_pointer_or_null nxt) && !!(~ ((x : val) = nullval)) && !!((s : list Z) = (([(v : Z)] : list Z) ++ (s1 : list Z))) && (data_at Tsh (tarray (Tunion _sslval noattr) 2) [(inl ((Vint (Int.repr v)) : val)); (inr (nxt : val))] (x : val)) * (sll (nxt : val) (s1 : list Z) (_alpha_517 : sll_card))
 end.
 
 
@@ -70,14 +70,15 @@ Definition tree_copy_spec :=
    SEP ((data_at Tsh (tarray (Tunion _sslval noattr) 1) [(inr (x : val))] (r : val)); (tree (x : val) (s : list Z) (a : tree_card)))
    POST[ tvoid ]
    EX y: val,
-   PROP(  )
+   PROP( is_pointer_or_null((y : val)) )
    LOCAL()
-   SEP ((data_at Tsh (tarray (Tunion _sslval noattr) 1) [(inr (y : val))] (r : val)); (tree (y : val) (s : list Z) (a : tree_card)); (tree (x : val) (s : list Z) (a : tree_card))).
+   SEP ((data_at Tsh (tarray (Tunion _sslval noattr) 1) [(inr (y : val))] (r : val)); (tree (x : val) (s : list Z) (a : tree_card)); (tree (y : val) (s : list Z) (a : tree_card))).
 
-Lemma tree_x_valid_pointerP x s self_card: tree x s self_card |-- valid_pointer x. Proof. Admitted.
+Lemma tree_x_valid_pointerP x s self_card: tree x s self_card |-- valid_pointer x. Proof. destruct self_card; simpl; entailer;  entailer!; eauto. Qed.
 Hint Resolve tree_x_valid_pointerP : valid_pointer.
 Lemma tree_local_factsP x s self_card :
-  tree x s self_card|-- !!(((((x : val) = nullval)) -> (self_card = tree_card_0))/\(((~ ((x : val) = nullval))) -> (exists _alpha_514 _alpha_513, self_card = tree_card_2 _alpha_514 _alpha_513))/\is_pointer_or_null((x : val))). Proof. Admitted.
+  tree x s self_card|-- !!(((((x : val) = nullval)) -> (self_card = tree_card_0))/\(((~ ((x : val) = nullval))) -> (exists _alpha_514 _alpha_513, self_card = tree_card_2 _alpha_514 _alpha_513))/\is_pointer_or_null((x : val))).
+ Proof.  destruct self_card;  simpl; entailer; saturate_local; apply prop_right; eauto. Qed.
 Hint Resolve tree_local_factsP : saturate_local.
 Lemma unfold_tree_card_0  (x: val) (s: (list Z)) : tree x s (tree_card_0 ) =  !!((x : val) = nullval) && !!((s : list Z) = ([] : list Z)) && emp. Proof. auto. Qed.
 Lemma unfold_tree_card_2 (_alpha_514 : tree_card) (_alpha_513 : tree_card) (x: val) (s: (list Z)) : tree x s (tree_card_2 _alpha_514 _alpha_513) = 
@@ -86,11 +87,12 @@ Lemma unfold_tree_card_2 (_alpha_514 : tree_card) (_alpha_513 : tree_card) (x: v
       EX r : val,
       EX s1 : (list Z),
       EX l : val,
- !!(Int.min_signed <= v <= Int.max_signed) && !!(~ ((x : val) = nullval)) && !!((s : list Z) = ((([(v : Z)] : list Z) ++ (s1 : list Z)) ++ (s2 : list Z))) && (data_at Tsh (tarray (Tunion _sslval noattr) 3) [(inl ((Vint (Int.repr v)) : val)); (inr (l : val)); (inr (r : val))] (x : val)) * (tree (r : val) (s2 : list Z) (_alpha_514 : tree_card)) * (tree (l : val) (s1 : list Z) (_alpha_513 : tree_card)). Proof. auto. Qed.
-Lemma treeN_x_valid_pointerP x n self_card: treeN x n self_card |-- valid_pointer x. Proof. Admitted.
+ !!(Int.min_signed <= v <= Int.max_signed) && !!(is_pointer_or_null r) && !!(is_pointer_or_null l) && !!(~ ((x : val) = nullval)) && !!((s : list Z) = ((([(v : Z)] : list Z) ++ (s1 : list Z)) ++ (s2 : list Z))) && (data_at Tsh (tarray (Tunion _sslval noattr) 3) [(inl ((Vint (Int.repr v)) : val)); (inr (l : val)); (inr (r : val))] (x : val)) * (tree (l : val) (s1 : list Z) (_alpha_513 : tree_card)) * (tree (r : val) (s2 : list Z) (_alpha_514 : tree_card)). Proof. auto. Qed.
+Lemma treeN_x_valid_pointerP x n self_card: treeN x n self_card |-- valid_pointer x. Proof. destruct self_card; simpl; entailer;  entailer!; eauto. Qed.
 Hint Resolve treeN_x_valid_pointerP : valid_pointer.
 Lemma treeN_local_factsP x n self_card :
-  treeN x n self_card|-- !!(((((x : val) = nullval)) -> (self_card = treeN_card_0))/\(((~ ((x : val) = nullval))) -> (exists _alpha_516 _alpha_515, self_card = treeN_card_2 _alpha_516 _alpha_515))/\is_pointer_or_null((x : val))). Proof. Admitted.
+  treeN x n self_card|-- !!(((((x : val) = nullval)) -> (self_card = treeN_card_0))/\(((~ ((x : val) = nullval))) -> (exists _alpha_516 _alpha_515, self_card = treeN_card_2 _alpha_516 _alpha_515))/\is_pointer_or_null((x : val))).
+ Proof.  destruct self_card;  simpl; entailer; saturate_local; apply prop_right; eauto. Qed.
 Hint Resolve treeN_local_factsP : saturate_local.
 Lemma unfold_treeN_card_0  (x: val) (n: Z) : treeN x n (treeN_card_0 ) =  !!((x : val) = nullval) && !!((n : Z) = 0) && emp. Proof. auto. Qed.
 Lemma unfold_treeN_card_2 (_alpha_516 : treeN_card) (_alpha_515 : treeN_card) (x: val) (n: Z) : treeN x n (treeN_card_2 _alpha_516 _alpha_515) = 
@@ -99,18 +101,19 @@ Lemma unfold_treeN_card_2 (_alpha_516 : treeN_card) (_alpha_515 : treeN_card) (x
       EX r : val,
       EX n2 : Z,
       EX l : val,
- !!(Int.min_signed <= n1 <= Int.max_signed) && !!(Int.min_signed <= n2 <= Int.max_signed) && !!(~ ((x : val) = nullval)) && !!(0 <= (n1 : Z)) && !!(0 <= (n2 : Z)) && !!((n : Z) = ((1 + (n1 : Z)) + (n2 : Z))) && (data_at Tsh (tarray (Tunion _sslval noattr) 3) [(inr (v : val)); (inr (l : val)); (inr (r : val))] (x : val)) * (treeN (r : val) (n2 : Z) (_alpha_516 : treeN_card)) * (treeN (l : val) (n1 : Z) (_alpha_515 : treeN_card)). Proof. auto. Qed.
-Lemma sll_x_valid_pointerP x s self_card: sll x s self_card |-- valid_pointer x. Proof. Admitted.
+ !!(Int.min_signed <= n1 <= Int.max_signed) && !!(is_pointer_or_null v) && !!(is_pointer_or_null r) && !!(Int.min_signed <= n2 <= Int.max_signed) && !!(is_pointer_or_null l) && !!(~ ((x : val) = nullval)) && !!(0 <= (n1 : Z)) && !!(0 <= (n2 : Z)) && !!((n : Z) = ((1 + (n1 : Z)) + (n2 : Z))) && (data_at Tsh (tarray (Tunion _sslval noattr) 3) [(inr (v : val)); (inr (l : val)); (inr (r : val))] (x : val)) * (treeN (l : val) (n1 : Z) (_alpha_515 : treeN_card)) * (treeN (r : val) (n2 : Z) (_alpha_516 : treeN_card)). Proof. auto. Qed.
+Lemma sll_x_valid_pointerP x s self_card: sll x s self_card |-- valid_pointer x. Proof. destruct self_card; simpl; entailer;  entailer!; eauto. Qed.
 Hint Resolve sll_x_valid_pointerP : valid_pointer.
 Lemma sll_local_factsP x s self_card :
-  sll x s self_card|-- !!(((((x : val) = nullval)) -> (self_card = sll_card_0))/\(((~ ((x : val) = nullval))) -> (exists _alpha_517, self_card = sll_card_1 _alpha_517))/\is_pointer_or_null((x : val))). Proof. Admitted.
+  sll x s self_card|-- !!(((((x : val) = nullval)) -> (self_card = sll_card_0))/\(((~ ((x : val) = nullval))) -> (exists _alpha_517, self_card = sll_card_1 _alpha_517))/\is_pointer_or_null((x : val))).
+ Proof.  destruct self_card;  simpl; entailer; saturate_local; apply prop_right; eauto. Qed.
 Hint Resolve sll_local_factsP : saturate_local.
 Lemma unfold_sll_card_0  (x: val) (s: (list Z)) : sll x s (sll_card_0 ) =  !!((x : val) = nullval) && !!((s : list Z) = ([] : list Z)) && emp. Proof. auto. Qed.
 Lemma unfold_sll_card_1 (_alpha_517 : sll_card) (x: val) (s: (list Z)) : sll x s (sll_card_1 _alpha_517) = 
       EX v : Z,
       EX s1 : (list Z),
       EX nxt : val,
- !!(Int.min_signed <= v <= Int.max_signed) && !!(~ ((x : val) = nullval)) && !!((s : list Z) = (([(v : Z)] : list Z) ++ (s1 : list Z))) && (data_at Tsh (tarray (Tunion _sslval noattr) 2) [(inl ((Vint (Int.repr v)) : val)); (inr (nxt : val))] (x : val)) * (sll (nxt : val) (s1 : list Z) (_alpha_517 : sll_card)). Proof. auto. Qed.
+ !!(Int.min_signed <= v <= Int.max_signed) && !!(is_pointer_or_null nxt) && !!(~ ((x : val) = nullval)) && !!((s : list Z) = (([(v : Z)] : list Z) ++ (s1 : list Z))) && (data_at Tsh (tarray (Tunion _sslval noattr) 2) [(inl ((Vint (Int.repr v)) : val)); (inr (nxt : val))] (x : val)) * (sll (nxt : val) (s1 : list Z) (_alpha_517 : sll_card)). Proof. auto. Qed.
 Definition Gprog : funspecs :=
   ltac:(with_library prog [tree_copy_spec; malloc_spec]).
 
@@ -131,9 +134,9 @@ let ssl_var := fresh in assert_PROP(s = ([] : list Z)) as ssl_var; try rewrite s
 forward; entailer!.
 Exists nullval.
 ssl_entailer.
-ssl_rewrite_last (unfold_tree_card_0 ).
+rewrite (unfold_tree_card_0 ) at 1.
 ssl_entailer.
-ssl_rewrite_last (unfold_tree_card_0 ).
+rewrite (unfold_tree_card_0 ) at 1.
 ssl_entailer.
 
 }
@@ -154,8 +157,8 @@ assert_PROP(is_pointer_or_null((r : val))). { entailer!. }
 assert_PROP(is_pointer_or_null((lx22 : val))). { entailer!. }
 forward_call ((r : val), (lx22 : val), (s1x2 : list Z), (_alpha_513x2 : tree_card)).
 Intros y1.
-assert_PROP(is_pointer_or_null((y1 : val))). { entailer!. }
 assert_PROP(is_pointer_or_null((lx22 : val))). { entailer!. }
+assert_PROP(is_pointer_or_null((y1 : val))). { entailer!. }
 try rename y1 into y12.
 forward.
 forward.
@@ -163,8 +166,8 @@ assert_PROP(is_pointer_or_null((r : val))). { entailer!. }
 assert_PROP(is_pointer_or_null((rx22 : val))). { entailer!. }
 forward_call ((r : val), (rx22 : val), (s2x2 : list Z), (_alpha_514x2 : tree_card)).
 Intros y2.
-assert_PROP(is_pointer_or_null((y2 : val))). { entailer!. }
 assert_PROP(is_pointer_or_null((rx22 : val))). { entailer!. }
+assert_PROP(is_pointer_or_null((y2 : val))). { entailer!. }
 try rename y2 into y22.
 forward.
 forward_call (tarray (Tunion _sslval noattr) 3).
@@ -177,14 +180,14 @@ forward.
 forward; entailer!.
 Exists (y3 : val).
 ssl_entailer.
-ssl_rewrite_last (unfold_tree_card_2 (_alpha_514x2 : tree_card) (_alpha_513x2 : tree_card)).
+rewrite (unfold_tree_card_2 (_alpha_514x2 : tree_card) (_alpha_513x2 : tree_card)) at 1.
 Exists (vx22 : Z).
 Exists (s2x2 : list Z).
 Exists (rx22 : val).
 Exists (s1x2 : list Z).
 Exists (lx22 : val).
 ssl_entailer.
-ssl_rewrite_last (unfold_tree_card_2 (_alpha_514x2 : tree_card) (_alpha_513x2 : tree_card)).
+rewrite (unfold_tree_card_2 (_alpha_514x2 : tree_card) (_alpha_513x2 : tree_card)) at 1.
 Exists (vx22 : Z).
 Exists (s2x2 : list Z).
 Exists (y22 : val).
